trying to prove termination mgu

mgu.fst
@@ -2,6 +2,8 @@ module Mgu
 
 open Term
 open Subst
+open FStar.Set
+open Union
 
 val apply_tuple_list : st:subst -> l:list (term*term) -> Tot (list (term*term))
 
@@ -27,9 +29,8 @@ let rec collate l1 l2 = match l1,l2 with
 
 let rec is_Unifiable*)
 
-val get_list_of_vars : term -> list variable -> Tot (list variable)
+(*val get_list_of_vars : term -> list variable -> Tot (list variable)
 val get_list_of_vars_list : list term -> list variable -> Tot (list variable)
-val get_list_of_vars_tuples : list (term*term) -> list variable -> Tot (list variable)
 
 let rec get_list_of_vars t lv =
   match t with
@@ -41,11 +42,22 @@ and get_list_of_vars_list lt lv = match lt with
   | hd::tl -> begin
                 let temp1 = get_list_of_vars hd lv in
                 get_list_of_vars_list tl temp1
-              end
+              end*)
 
-(*let rec get_list_of_vars_tuples ltt lv = match ltt with
-  | [] -> []
-  | (hd1,hd2)::tl -> *)
+val get_num_vars : term -> set variable -> Tot (nat*(set variable))
+val get_num_vars_list : list term -> set variable  -> Tot (nat*(set variable))
+
+let rec get_num_vars t sv = match t with
+  | Var v -> if mem v sv then (0,sv) else  (1,(union sv (singleton v)))
+  | Name n -> (0,sv)
+  | Func s args -> get_num_vars_list args sv
+and get_num_vars_list lt sv = match lt with
+  | [] -> (0,empty)
+  | hd::tl -> begin
+              let temp1 = get_num_vars hd sv in
+              let temp2 = (get_num_vars_list tl (snd temp1)) in
+              ((fst temp1)+(fst temp2),(snd temp2))
+              end
 
 val get_num_symbols : t:term -> Tot nat
 val get_num_symbols_list : lt:list term-> Tot nat
@@ -59,21 +71,58 @@ and get_num_symbols_list lt = match lt with
   | [] -> 0
   | hd::tl -> get_num_symbols hd + get_num_symbols_list tl
 
+val get_num_vars_tuple_list : list (term*term) -> set variable -> Tot nat
+
+let rec get_num_vars_tuple_list ltt sv = match ltt with
+  | [] -> 0
+  | (hd1,hd2)::tl -> let temp1 = get_num_vars hd1 sv in
+                    let temp2 = get_num_vars hd2 (snd temp1) in
+                    (fst temp1) + (fst temp2) + (get_num_vars_tuple_list tl (snd temp2))
+
 val rearrange_tuple_list : #a:eqtype -> list(a*a) -> Tot (list a)
 
 let rec rearrange_tuple_list #a l = match l with
   | [] -> []
   | (x,y)::tl -> x::(y::(rearrange_tuple_list tl))
 
-val aux_lemma1 : v:variable -> x:term -> ltt:list (term*term) -> Lemma
-  (requires true)
-  (ensures List.Tot.length(get_list_of_vars_list (rearrange_tuple_list (apply_tuple_list [(v,x)] ltt)) []) < List.Tot.length(get_list_of_vars_list (rearrange_tuple_list ((Var v,x)::ltt)) []) )
 
-let rec aux_lemma1 v x ltt = match ltt with
+val aux_lemma1a : t:term -> sv1:set variable -> sv2:set variable -> Lemma (requires true) (ensures (subset sv1 sv2  ==> (fst (get_num_vars t sv1) >= fst (get_num_vars t sv2))))
+val aux_lemma1b : lt:list term -> sv1:set variable -> sv2:set variable -> Lemma
+  (requires subset sv1 sv2)
+  (ensures (fst (get_num_vars_list lt sv1) >= fst (get_num_vars_list lt sv2)))
+val aux_lemma1e : t:term -> sv:set variable -> Lemma (requires true)(ensures (subset (sv) (snd (get_num_vars t sv))))
+val aux_lemma1f : lt:list term -> sv:set variable -> Lemma (requires true)(ensures (subset (sv) (snd (get_num_vars_list lt sv))))
+let rec aux_lemma1e t sv = match t with
+  | Var v -> ()
+  | Name n -> ()
+  | Func s args -> aux_lemma1f args sv
+and aux_lemma1f lt sv = match lt with
   | [] -> ()
-  | hd::tl -> admit()
+  | hd::tl -> aux_lemma1e hd sv
 
-val sub_mgu : l:list (term*term) -> st:subst -> Tot (option subst) (decreases %[(List.Tot.length(get_list_of_vars_list (rearrange_tuple_list l) []));(get_num_symbols_list (rearrange_tuple_list l))])
+let rec aux_lemma1a t sv1 sv2 = match t with
+  | Var v -> if mem v sv1 then (assert (fst (get_num_vars t sv1) = 0); assert (fst (get_num_vars t sv2) = 0))
+             else if mem v sv2 then (assert (fst (get_num_vars t sv1) = 1); assert (fst (get_num_vars t sv2) = 0))
+             else (assert (fst (get_num_vars t sv1) = 1); assert (fst (get_num_vars t sv2) = 1))
+  | Name n -> (assert (fst (get_num_vars t sv1) = 0); assert (fst (get_num_vars t sv2) = 0))
+  | Func s args -> aux_lemma1b args sv1 sv2
+and aux_lemma1b lt sv1 sv2 = match lt with
+  | [] -> ()
+  | hd::tl -> aux_lemma1a hd sv1 sv2 ;aux_lemma1b tl sv1 sv2
+
+val aux_lemma2 : hd1:term -> hd2:term -> tl:list (term*term) -> Lemma
+  (requires true)
+  (ensures get_num_vars_tuple_list ((hd1,hd2)::tl) empty <= fst (get_num_vars hd1 empty) + fst (get_num_vars hd2 empty) + get_num_vars_tuple_list tl empty)
+
+let aux_lemma2 hd1 hd2 tl= ()
+
+val aux_lemma9 : v:variable -> x:term -> ltt:list (term*term) -> Lemma
+  (requires true)
+  (ensures get_num_vars_tuple_list (apply_tuple_list [(v,x)] ltt) empty < get_num_vars_tuple_list ((Var v,x)::ltt) empty)
+
+let rec aux_lemma9 v x ltt = admit()
+
+val sub_mgu : l:list (term*term) -> st:subst -> Tot (option subst) (decreases %[get_num_vars_tuple_list l empty;(get_num_symbols_list (rearrange_tuple_list l))])
 let rec sub_mgu l st = match l with
   | [] -> Some st
   | (Var v, x)::tl
@@ -82,7 +131,7 @@ let rec sub_mgu l st = match l with
                         else (
                           let temp1 = (compose st [(v,x)]) in
                           let temp2 = (apply_tuple_list [(v,x)] tl) in
-                          aux_lemma1 v x tl;
+                          aux_lemma9 v x tl;
                           if None? (sub_mgu temp2 temp1) then None
                           else (sub_mgu temp2 temp1)
                         )
