union.fst
@@ -2,12 +2,20 @@ module Union
 
 open FStar.Set
 
-val union_lemma1 : #a:eqtype -> l1:set a -> l2:set a -> Lemma
-(requires (subset l1 l2))
-(ensures (union l1 l2 = l2)) [SMTPat (union l1 l2)]
+val union_lemma1 : #a:eqtype -> s1:set a -> s2:set a -> Lemma
+(requires (subset s1 s2))
+(ensures (equal (union s1 s2) s2)) [SMTPat (FStar.Set.union s1 s2)]
 
-let rec union_lemma1 #a l1 l2 = ()
+let rec union_lemma1 #a s1 s2 = ()
 
-(*val union_lemma2 : #a:eqtype -> l1:list a -> l2:list a -> Lemma (requires true) (ensures (union l1 l2 = union l2 l1))
+val union_lemma2 : #a :eqtype -> s1:set a -> s2:set a -> s3:set a -> Lemma (requires true)( ensures (equal (union s1 (union s2 s3)) (union s2 (union s1 s3))) ) [SMTPat (FStar.Set.union s1 (union s2 s3))]
 
-let rec union_lemma2 #a l1 l2 =*)
+let union_lemma2 #a s1 s2 s3 = ()
+
+val union_lemma3 : #a:eqtype -> s1:set a -> s2:set a -> Lemma (requires true) (ensures (equal (union s1 s2) (union s2 s1))) [SMTPat (FStar.Set.union s1 s2)]
+
+let rec union_lemma3 #a s1 s2 = ()
+
+val union_lemma4 : #a:eqtype -> s1:set a -> s2:set a -> Lemma (requires true) (ensures ( (equal s1 s2) ==> (equal s1 (union s1 s2)) )) [SMTPat (FStar.Set.union s1 s2)]
+
+let union_lemma4 #a s1 s2 = ()
